finish

src/Init/Data/Array/Lemmas.lean
@@ -3253,9 +3253,11 @@ theorem back!_eq_back? [Inhabited α] (a : Array α) : a.back! = a.back?.getD de
 @[simp] theorem back!_push [Inhabited α] (a : Array α) : (a.push x).back! = x := by
   simp [back!_eq_back?]
 
-theorem mem_of_back?_eq_some {xs : Array α} {a : α} (h : xs.back? = some a) : a ∈ xs := by
+theorem mem_of_back? {xs : Array α} {a : α} (h : xs.back? = some a) : a ∈ xs := by
   cases xs
-  simpa using List.mem_of_getLast?_eq_some (by simpa using h)
+  simpa using List.mem_of_getLast? (by simpa using h)
+
+@[deprecated mem_of_back? (since := "2024-10-21")] abbrev mem_of_back?_eq_some := @mem_of_back?
 
 theorem getElem?_push_lt (a : Array α) (x : α) (i : Nat) (h : i < a.size) :
     (a.push x)[i]? = some a[i] := by
